src/program_proof/mpaxos/definitions.v
@@ -220,5 +220,31 @@ Definition is_Server (s:loc) γ γsrv : iProp Σ :=
   "#HmuInv" ∷ is_lock mpN mu (own_Server s γ γsrv)
   (* "#Hsys_inv" ∷ sys_inv γ *).
 
+Definition enterNewEpoch_post γsrv (acceptedEpoch epoch:u64) σ : iProp Σ:=
+  is_accepted_ro γsrv acceptedEpoch σ ∗
+  (∀ epoch', ⌜int.nat acceptedEpoch < int.nat epoch'⌝ -∗
+            ⌜int.nat epoch' ≤ int.nat epoch⌝ -∗
+            is_accepted_ro γsrv epoch' [])
+.
+
+Lemma wp_singleClerk__enterNewEpoch ck γ γsrv args_ptr args reply_ptr init_reply :
+  {{{
+        "#His_ck" ∷ is_singleClerk ck γ γsrv ∗
+        "Hargs" ∷ enterNewEpochArgs.own args_ptr args 1 ∗
+        "Hreply" ∷ enterNewEpochReply.own reply_ptr init_reply 1
+  }}}
+    singleClerk__enterNewEpoch #ck #args_ptr #reply_ptr
+  {{{
+        reply, RET #(); enterNewEpochReply.own reply_ptr reply 1 ∗
+        □if (decide (reply.(enterNewEpochReply.err) = (U64 0))) then
+          ∃ σ,
+          ⌜reply.(enterNewEpochReply.state) = get_state σ⌝ ∗
+          enterNewEpoch_post γsrv reply.(enterNewEpochReply.acceptedEpoch)
+                                          args.(enterNewEpochArgs.epoch) σ
+        else
+          True
+  }}}.
+Proof.
+Admitted.
 
 End definitions.
