src/program_proof/mpaxos/apply_proof.v
@@ -295,7 +295,6 @@ Proof.
       }
       done.
     }
-    done.
   }
 
   set (newstate:=(next_state (default [] (last st.(mp_log).*1)) op)).
