src/program_proof/mpaxos/becomeleader_proof.v
@@ -1,0 +1,131 @@
+From Perennial.program_proof Require Import grove_prelude.
+From Goose.github_com.mit_pdos.gokv Require mpaxos.
+From Perennial.program_proof.grove_shared Require Import urpc_proof urpc_spec.
+From Perennial.goose_lang.lib Require Import waitgroup.
+From iris.base_logic Require Export lib.ghost_var mono_nat.
+From iris.algebra Require Import dfrac_agree mono_list.
+From Perennial.goose_lang Require Import crash_borrow.
+From Perennial.program_proof Require Import marshal_stateless_proof.
+From Perennial.program_proof.mpaxos Require Export definitions.
+
+Section becomeleader_proof.
+
+Context `{!heapGS Σ}.
+Context {mp_record:MPRecord}.
+Notation OpType := (mp_OpType mp_record).
+Notation has_op_encoding := (mp_has_op_encoding mp_record).
+Notation next_state := (mp_next_state mp_record).
+Notation compute_reply := (mp_compute_reply mp_record).
+Notation is_Server := (is_Server (mp_record:=mp_record)).
+Notation is_singleClerk := (is_singleClerk (mp_record:=mp_record)).
+
+Context (conf:list mp_server_names).
+Context `{!mpG Σ}.
+
+Lemma wp_Server__becomeLeader s γ γsrv :
+  {{{
+        is_Server conf s γ γsrv
+  }}}
+    mpaxos.Server__becomeLeader #s
+  {{{
+        RET #(); True
+  }}}.
+Proof.
+  iIntros (Φ) "#Hsrv HΦ".
+  wp_call.
+  iNamed "Hsrv".
+  wp_loadField.
+  wp_apply (acquire_spec with "HmuInv").
+  iIntros "[Hlocked Hown]".
+  iNamed "Hown".
+
+  wp_pures.
+  wp_loadField.
+  wp_if_destruct.
+  { (* already leader, no need to do anything *)
+    admit.
+  }
+  wp_loadField.
+  wp_pures.
+  wp_loadField.
+  wp_apply (wp_allocStruct).
+  { repeat econstructor. }
+  iIntros (args_ptr) "Hargs".
+  wp_pures.
+  wp_loadField.
+  wp_apply (release_spec with "[-HΦ Hargs]").
+  {
+    iFrame "HmuInv Hlocked".
+    iNext.
+    iExists _,_,_,_,_,_.
+    iFrame "∗#%".
+  }
+
+  wp_pures.
+  wp_apply (wp_ref_to).
+  { eauto. }
+  iIntros (numReplies_ptr) "HnumReplies".
+  wp_pures.
+
+  iMod (readonly_load with "Hclerks_sl") as (?) "Hclerks_sl2".
+  iDestruct (is_slice_small_sz with "Hclerks_sl2") as "%Hclerks_sz".
+  iClear "Hclerks_sl2".
+  clear q.
+
+  wp_apply (wp_slice_len).
+  wp_apply (wp_NewSlice).
+  iIntros (replies_sl) "Hreplies_sl".
+  wp_pures.
+  rewrite -Hclerks_sz.
+
+  set (newepoch:=word.add st.(mp_epoch) 1).
+  set (replyInv:=(
+                  ∃ (numReplies:u64) (reply_ptrs:list loc),
+                    "HnumReplies" ∷ numReplies_ptr ↦[uint64T] #numReplies ∗
+                    "Hreplies_sl" ∷ is_slice_small replies_sl ptrT 1 reply_ptrs ∗
+                    "#Hreplies" ∷ ([∗ list] i ↦ reply_ptr ; γsrv' ∈ reply_ptrs ; conf,
+                    ⌜reply_ptr = null⌝ ∨ (∃ reply σ, enterNewEpochReply.own reply_ptr reply 1 ∗
+                                              □(if decide (reply.(enterNewEpochReply.err) = (U64 0)) then
+                                                enterNewEpoch_post γsrv reply.(enterNewEpochReply.acceptedEpoch)
+                                                                                newepoch σ
+                                              else
+                                                True)
+                                  ))
+                )%I).
+  wp_apply (newlock_spec mpN _ replyInv with "[HnumReplies Hreplies_sl]").
+  {
+    iNext.
+    iExists _, _.
+    iDestruct (is_slice_to_small with "Hreplies_sl") as "$".
+    iFrame "∗".
+    iDestruct (big_sepL2_length with "Hclerks_rpc") as "%Hlen".
+    iApply big_sepL2_impl.
+    {
+      instantiate (1:=(λ _ _ _, True)%I).
+      simpl.
+      iApply big_sepL2_forall.
+      iIntros.
+      iSplit.
+      {
+        iPureIntro.
+        rewrite Hlen.
+        by rewrite replicate_length.
+      }
+      done.
+    }
+    iModIntro.
+    iIntros.
+    iLeft.
+    rewrite lookup_replicate in H.
+    naive_solver.
+  }
+  iIntros (muReply) "#HmuReplyInv".
+  wp_pures.
+  wp_apply (wp_newCond with "HmuReplyInv").
+  iIntros (numReplies_cond) "HnumReplies_cond".
+  wp_pures.
+  wp_apply (wp_slice_len).
+  wp_pures.
+Admitted.
+
+End becomeleader_proof.
